<section xml:id="sec-integer_exponents">
  <title>Integer Exponents</title>
  <introduction>
    <p>
      For a non-negative integer <m>n</m>:
      <ul>
        <li>
          <p>
            The notation <m>a^n</m> represents <m>a</m> multiplied by itself <m>n</m> times. ex:
            <m>5^3 = 5 \times 5 \times 5</m>.
          </p>
        </li>
        <li>
          <p>
            If <m>a \neq 0</m>,
            then <m>a^0 = 1</m> because <m>a</m> multiplied by itself zero times is a product that has no terms,
            and a product that has no terms equals <m>1</m>.
            Note: <m>0^0</m> is not a number;
            it is an indeterminate form that will be studied in calculus.
          </p>
        </li>
        <li>
          <p>
            <em>Multiplying exponents:</em>
            When multiplying powers of the same base,
            add the exponents, because:
            <me>
              a^n  \times a^m = \underbrace{aa\cdots a}_{n\ \mathrm{times}}  \times \underbrace{aa\cdots a}_{m\ \mathrm{times} } = \underbrace{aa\cdots a \times aa\cdots a}_{n+m\ \mathrm{times} } = a^{n+m}
            </me>
            When multiplying exponential expressions of different bases but of the same power,
            multiply by the bases together and raise it to the exponent, because:
            <me>
              a^n\times b^n = \underbrace{aa\cdots a}_{n\ \mathrm{times}}  \times \underbrace{bb\cdots b}_{n\ \mathrm{times} } = \underbrace{abab \cdots ab}_{n\ \mathrm{times} } = (ab)^n
            </me>
          </p>
        </li>
        <li>
          <p>
            <em>Powers of Powers:</em> When raising a power to another power,
            multiply the exponents, because:
            <me>
              (a^n)^m  =  \underbrace{a^n a^n\cdots a^n}_{m\ \mathrm{times}}= \underbrace{aaaa\cdots aaa \times aaa\cdots aa}_{nm\ \mathrm{times} } =  a^{nm}
            </me>
          </p>
        </li>
        <li>
          <p>
            <em>Negative exponents</em> are a shorthand for a power of the reciprocal,
            and only make sense if the base is not zero.
            That is, for <m>n > 0</m> and <m>a \neq 0</m>,
            <me>
              a^{-n} =  \big( a^{-1} \big)^n = \left( \frac{1}{a} \right)^n= \frac{1}{a^n}
            </me>.
            Note that  <m>a^{-1} = \frac{1}{a}</m>.
          </p>
        </li>
        <li>
          <p>
            <em>Dividing exponents:</em> When dividing powers of the same base,
            subtract the exponents because of the meaning of negative exponents (above):
            <me>
              a^n \div a^m = \frac{a^n}{a^m}= a^n\left(\frac{1}{a^m}\right)= a^n \times a^{-m} =  a^{n-m}
            </me>.
          </p>
        </li>
        <li>
          <p>
            If you have different bases to different powers,
            sometimes you can combine by factoring.
            See below.
          </p>
        </li>
      </ul>
    </p>
    <example>
      <statement>
        <ul>
          <li>
            <p>
              <m>6^3 \cdot 6^7 = 6^{3+7} = 6^{10}</m>
            </p>
          </li>
          <li>
            <p>
              <m>2^4 \cdot 2^7 = 2^{4+7} = 2^{11}</m>.
              Notice that <m>2^{11}</m> can arise other ways;
              for example <m>2^{11} =2^{8+3} = 2^8 \cdot 2^3</m>
            </p>
          </li>
          <li>
            <p>
              <m>(4^{60})^2 = 4^{60 \times 2} = 4^{120}</m>
            </p>
          </li>
          <li>
            <p>
              <m>\frac{1}{343} = \frac{1}{7^3} = 7^{-3}</m>
            </p>
          </li>
          <li>
            <p>
              <m>9^6 \div 9^2 = 9^{6-2} = 9^{4}</m>
            </p>
          </li>
          <li>
            <p>
              <m>\frac{3^{-4}}{3^{-5}} = 3^{-4- (-5 )} = 3^1 = 3</m>
            </p>
          </li>
          <li>
            <p>
              <m>4^3 5^3 =(4 \times 5)^3 = 20^{3}</m>
            </p>
          </li>
          <li>
            <p>
              <m>2^5 \cdot 8^6 = 2^5 \cdot (2^3)^6 = 2^5 \cdot 2^{18} = 2^{23}</m>
            </p>
          </li>
          <li>
            <p>
              <m>3^2 \cdot 9^{-4} = 3^2 \cdot (3^2)^{-4} = 3^2 \cdot (3^{-8}) = 3^{-6}</m>
            </p>
          </li>
          <li>
            <p>
              <m>(35)^2 \cdot 7^9 = (5\cdot 7)^2 \cdot 7^{9} = 5^2 \cdot 7^{11}</m>
            </p>
          </li>
          <li>
            <p>
              <m>12^3 \cdot 18^4 = (2\cdot 6)^3 \cdot (3\cdot 6)^4 = 2^3\cdot 6^3\cdot 3^4 \cdot 6^4 = 2^3\cdot 3^4 \cdot 6^7 = 3\cdot 6^3\cdot 6^7= 3\cdot 6^{10}</m>
            </p>
          </li>
        </ul>
      </statement>
    </example>
  </introduction>
  <subsection>
    <title>Practice Problems</title>
    <p>
      Use the rules of exponents to find an expression equivalent to the following:
      <ol>
        <li>
          <p>
            <m>z^4 \cdot z^{-5}</m>
          </p>
        </li>
        <li>
          <p>
            <m>(9^3)^4</m>
          </p>
        </li>
        <li>
          <p>
            <m>(2^{-2})^{-4}</m>
          </p>
        </li>
        <li>
          <p>
            <m>\frac{q^5}{q^2}</m>
          </p>
        </li>
        <li>
          <p>
            <m>(-4)^3 \cdot 5^3</m>
          </p>
        </li>
      </ol>
    </p>
  </subsection>
  <subsection>
    <title>Solutions</title>
    <p>
      1. <m>z^{-1}</m> 2.
      <m>9^{12} = 3^{24}</m> 3.
      <m>2^8</m> 4. <m>q^3</m> 5. <m>(-20)^3 = - (20^3) = -20^3</m>
    </p>
    <p>
      In each case there are other correct solutions.
    </p>
  </subsection>
</section>